Minterm.thy
@@ -8,9 +8,34 @@ text {* This section contains the minterms definition and some propositions rela
 
 theory Minterm
 imports
+  Formula_Relation 
   Test_Formulae
 begin
 
 
 subsection {* Definition *}
 
+typedef ('var, 'addr, 'k::finite) minterm 
+  = "{S. (\<exists>!l\<in>S::('var, 'k::finite) literal set. \<exists>n. (equivalence (UNIV::'addr set) (to_sl_formula l) (ext_card_heap_superior_to n)))}"
+proof 
+  define x::"('var, 'k::finite) literal set" where "x = {to_literal (ext_card_heap_superior_to 0)}"
+  show "x\<in>{S. \<exists>!l. l \<in> S \<and> (\<exists>n. equivalence UNIV (to_sl_formula l) (ext_card_heap_superior_to n))} "
+  proof
+oops
+
+(*
+definition minterm :: "'addr set \<Rightarrow> ('var, 'k::finite) literal set \<Rightarrow> bool"
+  where "minterm env S = ((\<exists>!l\<in>S. \<exists>n. (equivalence env (to_sl_formula l) (ext_card_heap_superior_to n)))
+                        \<and> (\<exists>!l\<in>S. \<exists>n. (equivalence env (to_sl_formula l) (not (ext_card_heap_superior_to n)))))"
+
+definition e_minterm
+  where ""
+*)
+
+(* 3 lemmes:
+- si minterm \<Rightarrow> a
+- si minterm \<Rightarrow> b
+- si a et b \<Rightarrow> mintern
+*)
+
+end
